src/opt/ReorderFence.v
@@ -48,6 +48,47 @@ Inductive sim_fence: forall (st_src:lang.(Language.state)) (th_src:Local.t) (mem
       (State.mk rs [Stmt.instr i2]) th1_tgt mem_k_tgt
 .
 
+Lemma sim_fence_step
+      st1_src th1_src mem_k_src
+      st1_tgt th1_tgt mem_k_tgt
+      (SIM: sim_fence st1_src th1_src mem_k_src
+                      st1_tgt th1_tgt mem_k_tgt):
+  forall mem1_src mem1_tgt
+    (MEMORY: sim_memory mem1_src mem1_tgt)
+    (FUTURE_SRC: Memory.future mem_k_src mem1_src)
+    (FUTURE_TGT: Memory.future mem_k_tgt mem1_tgt)
+    (WF_SRC: Local.wf th1_src mem1_src)
+    (WF_TGT: Local.wf th1_tgt mem1_tgt),
+    _sim_thread_step lang lang ((sim_thread (sim_terminal eq)) \6/ sim_fence)
+                     st1_src th1_src mem1_src
+                     st1_tgt th1_tgt mem1_tgt.
+Proof.
+  inv SIM. ii.
+  exploit Local.future_fence_step; try apply FENCE; eauto. i.
+  inv STEP_TGT; inv STEP; try (inv STATE; inv INSTR; inv REORDER); ss.
+  - (* promise *)
+    exploit sim_local_promise; eauto.
+    { eapply Local.fence_step_future; eauto. }
+    i. des.
+    exploit reorder_fence_promise; try apply x0; try apply STEP_SRC; eauto.
+    { inv REORDER; ss. }
+    { inv REORDER; ss. }
+    i. des.
+    eexists _, _, _, _, _, _. splits; eauto.
+    + econs. econs 1; eauto.
+    + right. econs; eauto.
+  - (* store *)
+    exploit sim_local_write; eauto.
+    { eapply Local.fence_step_future; eauto. }
+    i. des.
+    exploit reorder_fence_write; try apply x0; try apply STEP_SRC; eauto. i. des.
+    eexists _, _, _, _, _, _. splits.
+    + econs 2; [|econs 1]. econs 2. econs 3; eauto. econs. econs.
+    + econs 2. econs 5; eauto. econs. econs.
+    + s. eauto.
+    + s. left. eapply paco7_mon; [apply sim_stmts_nil|]; ss.
+Qed.
+
 Lemma sim_fence_sim_thread:
   sim_fence <6= (sim_thread (sim_terminal eq)).
 Proof.
@@ -62,28 +103,8 @@ Proof.
   - i. eexists _, _, _. splits; eauto.
     inv PR. inv FENCE. inv LOCAL. ss.
     apply MemInv.sem_bot_inv in PROMISE. rewrite PROMISE. auto.
-  - inv PR. i. inv STEP_TGT; [|by inv STEP; inv STATE; inv INSTR; inv REORDER].
-    exploit Local.future_fence_step; try apply FENCE; eauto. i.
-    inv STEP; try (inv STATE; inv INSTR; inv REORDER); ss.
-    + (* promise *)
-      exploit sim_local_promise; eauto.
-      { eapply Local.fence_step_future; eauto. }
-      i. des.
-      exploit reorder_fence_promise; try apply x0; try apply STEP_SRC; eauto.
-      { inv REORDER; ss. }
-      { inv REORDER; ss. }
-      i. des.
-      eexists _, _, _, _, _, _. splits; eauto.
-      * econs. econs 1; eauto.
-      * right. apply CIH. econs; eauto.
-    + (* store *)
-      exploit sim_local_write; eauto.
-      { eapply Local.fence_step_future; eauto. }
-      i. des.
-      exploit reorder_fence_write; try apply x0; try apply STEP_SRC; eauto. i. des.
-      eexists _, _, _, _, _, _. splits.
-      * econs 2; [|econs 1]. econs 4; eauto. econs. econs.
-      * econs. econs 6; eauto. econs. econs.
-      * s. eauto.
-      * s. left. eapply paco7_mon; [apply sim_stmts_nil|]; ss.
+  - ii. exploit sim_fence_step; eauto. i. des.
+    + eexists _, _, _, _, _, _. splits; eauto.
+      left. eapply paco7_mon; eauto. ss.
+    + eexists _, _, _, _, _, _. splits; eauto.
 Qed.
