src/opt/ReorderLoad.v
@@ -70,6 +70,91 @@ Inductive sim_load: forall (st_src:lang.(Language.state)) (th_src:Local.t) (mem_
       (State.mk (RegFun.add r1 v1 rs) [Stmt.instr i2]) th1_tgt mem_k_tgt
 .
 
+Lemma sim_load_step
+      st1_src th1_src mem_k_src
+      st1_tgt th1_tgt mem_k_tgt
+      (SIM: sim_load st1_src th1_src mem_k_src
+                     st1_tgt th1_tgt mem_k_tgt):
+  forall mem1_src mem1_tgt
+    (MEMORY: sim_memory mem1_src mem1_tgt)
+    (FUTURE_SRC: Memory.future mem_k_src mem1_src)
+    (FUTURE_TGT: Memory.future mem_k_tgt mem1_tgt)
+    (WF_SRC: Local.wf th1_src mem1_src)
+    (WF_TGT: Local.wf th1_tgt mem1_tgt),
+    _sim_thread_step lang lang ((sim_thread (sim_terminal eq)) \6/ sim_load)
+                     st1_src th1_src mem1_src
+                     st1_tgt th1_tgt mem1_tgt.
+Proof.
+  inv SIM. ii.
+  exploit Local.future_read_step; try apply READ; eauto. i.
+  inv STEP_TGT; inv STEP; try (inv STATE; inv INSTR; inv REORDER); ss.
+  - (* promise *)
+    exploit sim_local_promise; eauto.
+    { eapply Local.read_step_future; eauto. }
+    i. des.
+    exploit reorder_read_promise; try apply x0; try apply STEP_SRC; eauto. i. des.
+    eexists _, _, _, _, _, _. splits; eauto.
+    + econs. econs 1; eauto.
+    + right. econs; eauto.
+  - (* load *)
+    exploit sim_local_read; eauto.
+    { eapply Local.read_step_future; eauto. }
+    i. des.
+    exploit reorder_read_read; try apply x0; try apply STEP_SRC; eauto. i. des.
+    eexists _, _, _, _, _, _. splits.
+    + econs 2; [|econs 1]. econs 2. econs 2; eauto. econs. econs.
+    + econs 2. econs 2; eauto. econs. econs.
+    + s. eauto.
+    + s. left. eapply paco7_mon; [apply sim_stmts_nil|]; ss.
+      apply RegFun.add_add. admit. (* singleton disjoint => neq *)
+  - (* store *)
+    exploit sim_local_write; eauto.
+    { eapply Local.read_step_future; eauto. }
+    i. des.
+    exploit reorder_read_write; try apply x0; try apply STEP_SRC; eauto. i. des.
+    eexists _, _, _, _, _, _. splits.
+    + econs 2; [|econs 1]. econs 2. econs 3; eauto. econs.
+      erewrite RegFile.eq_except_value; eauto.
+      * econs.
+      * apply RegFile.eq_except_singleton.
+    + econs 2. econs 2; eauto. econs. econs.
+    + s. eauto.
+    + s. left. eapply paco7_mon; [apply sim_stmts_nil|]; ss.
+  - (* update *)
+    exploit sim_local_read; eauto.
+    { eapply Local.read_step_future; eauto. }
+    i. des.
+    exploit sim_local_write; eauto.
+    { eapply Local.read_step_future; eauto.
+      eapply Local.read_step_future; eauto.
+    }
+    { eapply Local.read_step_future; eauto. }
+    i. des.
+    exploit reorder_read_read; try apply x0; try apply STEP_SRC; eauto. i. des.
+    exploit reorder_read_write; try apply STEP2; try apply LOCAL2; eauto.
+    { eapply Local.read_step_future; eauto. }
+    i. des.
+    eexists _, _, _, _, _, _. splits.
+    + econs 2; [|econs 1]. econs 2. econs 4; eauto. econs. econs.
+      erewrite <- RegFile.eq_except_rmw; eauto.
+      * admit. (* disjoint add => disjoint *)
+      * apply RegFile.eq_except_singleton.
+    + econs 2. econs 2; eauto. econs. econs.
+    + s. eauto.
+    + s. left. eapply paco7_mon; [apply sim_stmts_nil|]; ss.
+      apply RegFun.add_add. admit. (* disjoint singleton => neq *)
+  - (* fence *)
+    exploit sim_local_fence; eauto.
+    { eapply Local.read_step_future; eauto. }
+    i. des.
+    exploit reorder_read_fence; try apply x0; try apply STEP_SRC; eauto. i. des.
+    eexists _, _, _, _, _, _. splits.
+    + econs 2; [|econs 1]. econs 2. econs 5; eauto. econs. econs.
+    + econs 2. econs 2; eauto. econs. econs.
+    + s. eauto.
+    + s. left. eapply paco7_mon; [apply sim_stmts_nil|]; ss.
+Admitted.
+
 Lemma sim_load_sim_thread:
   sim_load <6= (sim_thread (sim_terminal eq)).
 Proof.
@@ -84,72 +169,8 @@ Proof.
   - i. eexists _, _, _. splits; eauto.
     inv PR. inv READ. inv LOCAL. ss.
     apply MemInv.sem_bot_inv in PROMISE. rewrite PROMISE. auto.
-  - inv PR. i. inv STEP_TGT; [|by inv STEP; inv STATE; inv INSTR; inv REORDER].
-    exploit Local.future_read_step; try apply READ; eauto. i.
-    inv STEP; try (inv STATE; inv INSTR; inv REORDER); ss.
-    + (* promise *)
-      exploit sim_local_promise; eauto.
-      { eapply Local.read_step_future; eauto. }
-      i. des.
-      exploit reorder_read_promise; try apply x0; try apply STEP_SRC; eauto. i. des.
-      eexists _, _, _, _, _, _. splits; eauto.
-      * econs. econs 1; eauto.
-      * right. apply CIH. econs; eauto.
-    + (* load *)
-      exploit sim_local_read; eauto.
-      { eapply Local.read_step_future; eauto. }
-      i. des.
-      exploit reorder_read_read; try apply x0; try apply STEP_SRC; eauto. i. des.
-      eexists _, _, _, _, _, _. splits.
-      * econs 2; [|econs 1]. econs 3; eauto. econs. econs.
-      * econs. econs 3; eauto. econs. econs.
-      * s. eauto.
-      * s. left. eapply paco7_mon; [apply sim_stmts_nil|]; ss.
-        apply RegFun.add_add. admit. (* singleton disjoint => neq *)
-    + (* store *)
-      exploit sim_local_write; eauto.
-      { eapply Local.read_step_future; eauto. }
-      i. des.
-      exploit reorder_read_write; try apply x0; try apply STEP_SRC; eauto. i. des.
-      eexists _, _, _, _, _, _. splits.
-      * econs 2; [|econs 1]. econs 4; eauto. econs.
-        erewrite RegFile.eq_except_value; eauto.
-        { econs. }
-        { apply RegFile.eq_except_singleton. }
-      * econs. econs 3; eauto. econs. econs.
-      * s. eauto.
-      * s. left. eapply paco7_mon; [apply sim_stmts_nil|]; ss.
-    + (* update *)
-      exploit sim_local_read; eauto.
-      { eapply Local.read_step_future; eauto. }
-      i. des.
-      exploit sim_local_write; eauto.
-      { eapply Local.read_step_future; eauto.
-        eapply Local.read_step_future; eauto.
-      }
-      { eapply Local.read_step_future; eauto. }
-      i. des.
-      exploit reorder_read_read; try apply x0; try apply STEP_SRC; eauto. i. des.
-      exploit reorder_read_write; try apply STEP2; try apply LOCAL2; eauto.
-      { eapply Local.read_step_future; eauto. }
-      i. des.
-      eexists _, _, _, _, _, _. splits.
-      * econs 2; [|econs 1]. econs 5; eauto. econs. econs.
-        erewrite <- RegFile.eq_except_rmw; eauto.
-        { admit. (* disjoint add => disjoint *) }
-        { apply RegFile.eq_except_singleton. }
-      * econs. econs 3; eauto. econs. econs.
-      * s. eauto.
-      * s. left. eapply paco7_mon; [apply sim_stmts_nil|]; ss.
-        { apply RegFun.add_add. admit. (* disjoint singleton => neq *) }
-    + (* fence *)
-      exploit sim_local_fence; eauto.
-      { eapply Local.read_step_future; eauto. }
-      i. des.
-      exploit reorder_read_fence; try apply x0; try apply STEP_SRC; eauto. i. des.
-      eexists _, _, _, _, _, _. splits.
-      * econs 2; [|econs 1]. econs 6; eauto. econs. econs.
-      * econs. econs 3; eauto. econs. econs.
-      * s. eauto.
-      * s. left. eapply paco7_mon; [apply sim_stmts_nil|]; ss.
-Admitted.
+  - ii. exploit sim_load_step; eauto. i. des.
+    + eexists _, _, _, _, _, _. splits; eauto.
+      left. eapply paco7_mon; eauto. ss.
+    + eexists _, _, _, _, _, _. splits; eauto.
+Qed.
