src/opt/ReorderStore.v
@@ -18,6 +18,7 @@ Require Import Configuration.
 Require Import Simulation.
 Require Import Compatibility.
 Require Import MemInv.
+Require Import Progress.
 Require Import ReorderBase.
 
 Require Import Syntax.
@@ -66,6 +67,87 @@ Inductive sim_store: forall (st_src:lang.(Language.state)) (th_src:Local.t) (mem
       (State.mk rs [Stmt.instr i2]) th1_tgt mem_k_tgt
 .
 
+Lemma sim_store_step
+      st1_src th1_src mem_k_src
+      st1_tgt th1_tgt mem_k_tgt
+      (SIM: sim_store st1_src th1_src mem_k_src
+                      st1_tgt th1_tgt mem_k_tgt):
+  forall mem1_src mem1_tgt
+    (MEMORY: sim_memory mem1_src mem1_tgt)
+    (FUTURE_SRC: Memory.future mem_k_src mem1_src)
+    (FUTURE_TGT: Memory.future mem_k_tgt mem1_tgt)
+    (WF_SRC: Local.wf th1_src mem1_src)
+    (WF_TGT: Local.wf th1_tgt mem1_tgt),
+    _sim_thread_step lang lang ((sim_thread (sim_terminal eq)) \6/ sim_store)
+                     st1_src th1_src mem1_src
+                     st1_tgt th1_tgt mem1_tgt.
+Proof.
+  inv SIM. ii.
+  exploit Local.future_fulfill_step; try apply FULFILL; eauto. i.
+  inv STEP_TGT; inv STEP; try (inv STATE; inv INSTR; inv REORDER).
+  - (* promise *)
+    exploit sim_local_promise; eauto.
+    { eapply Local.fulfill_step_future; eauto. }
+    i. des.
+    exploit reorder_fulfill_promise; try apply x0; try apply STEP_SRC; eauto. i. des.
+    eexists _, _, _, _, _, _. splits; eauto.
+    + econs 1. econs; eauto.
+    + right. econs; eauto.
+  - (* load *)
+    exploit sim_local_read; eauto.
+    { eapply Local.fulfill_step_future; eauto. }
+    i. des.
+    exploit reorder_fulfill_read; try apply x0; try apply STEP_SRC; eauto. i. des.
+    eexists _, _, _, _, _, _. splits.
+    + econs 2; [|econs 1]. econs 2. econs 2; eauto. econs. econs.
+    + econs 2. econs 3; eauto. econs.
+      * econs.
+      * s. econs 1. erewrite RegFile.eq_except_value; eauto.
+        { admit. (* RegSet.disjoint symmetry *) }
+        { apply RegFile.eq_except_singleton. }
+        { i. rewrite ORD1 in H. inv H. }
+    + eauto.
+    + left. eapply paco7_mon; [apply sim_stmts_nil|]; ss.
+  - (* store *)
+    exploit sim_local_write; eauto.
+    { eapply Local.fulfill_step_future; eauto. }
+    i. des.
+    exploit reorder_fulfill_write; try apply x0; try apply STEP_SRC; eauto.
+    i. des.
+    eexists _, _, _, _, _, _. splits.
+    + econs 2; [|econs 1]. econs 2. econs 3; eauto. econs. econs.
+    + econs 2. econs 3; eauto. econs.
+      * econs.
+      * s. econs 1; eauto.
+        i. rewrite ORD1 in H. inv H.
+    + s. eauto.
+    + s. left. eapply paco7_mon; [apply sim_stmts_nil|]; ss.
+  - (* update *)
+    exploit sim_local_read; eauto.
+    { eapply Local.fulfill_step_future; eauto. }
+    i. des.
+    exploit sim_local_write; eauto.
+    { eapply Local.read_step_future; eauto.
+      eapply Local.fulfill_step_future; eauto.
+    }
+    { eapply Local.read_step_future; eauto. }
+    i. des.
+    exploit reorder_fulfill_read; try apply x0; try apply STEP_SRC; eauto. i. des.
+    exploit reorder_fulfill_write; try apply STEP2; try apply STEP_SRC0; eauto.
+    { eapply Local.read_step_future; eauto. }
+    i. des.
+    eexists _, _, _, _, _, _. splits.
+    + econs 2; [|econs 1]. econs 2. econs 4; eauto. econs. econs. eauto.
+    + econs 2. econs 3; eauto.
+      * econs. econs.
+      * s. econs 1. erewrite RegFile.eq_except_value; eauto.
+        { admit. (* RegSet.disjoint symmetry *) }
+        { apply RegFile.eq_except_singleton. }
+        { i. rewrite ORD1 in H. inv H. }
+    +  s. eauto.
+    + s. left. eapply paco7_mon; [apply sim_stmts_nil|]; ss.
+Admitted.
+
 Lemma sim_store_sim_thread:
   sim_store <6= (sim_thread (sim_terminal eq)).
 Proof.
@@ -77,74 +159,26 @@ Proof.
     + eapply Local.fulfill_step_future; eauto.
       eapply Local.future_fulfill_step; eauto.
       eapply Local.future_fulfill_step; eauto.
-  - admit. (* promise *)
-    (* https://github.com/jeehoonkang/memory-model-explorer/blob/11e21b0c9147859fca4c63e0b21bdbac6dac6215/formalization/src/opt/ReorderWrite.v#L430 *)
-    (* https://github.com/jeehoonkang/memory-model-explorer/blob/86c803103989f87a17f50e6349aa9f285104af09/formalization/src/opt/Reorder.v#L116 *)
-  - inv PR. i. inv STEP_TGT; [|by inv STEP; inv STATE; inv INSTR; inv REORDER].
-    exploit Local.future_fulfill_step; try apply FULFILL; eauto. i.
-    inv STEP; try (inv STATE; inv INSTR; inv REORDER); ss.
-    + (* promise *)
-      exploit sim_local_promise; eauto.
-      { eapply Local.fulfill_step_future; eauto. }
-      i. des.
-      exploit reorder_fulfill_promise; try apply x0; try apply STEP_SRC; eauto. i. des.
-      eexists _, _, _, _, _, _. splits; eauto.
-      * econs. econs 1; eauto.
-      * right. apply CIH. econs; eauto.
-    + (* load *)
-      exploit sim_local_read; eauto.
-      { eapply Local.fulfill_step_future; eauto. }
-      i. des.
-      exploit reorder_fulfill_read; try apply x0; try apply STEP_SRC; eauto. i. des.
-      eexists _, _, _, _, _, _. splits.
-      * econs 2; [|econs 1]. econs 3; eauto. econs. econs.
-      * econs. econs 4; eauto. econs.
-        { econs. }
-        { s. econs 1. erewrite RegFile.eq_except_value; eauto.
-          - admit. (* RegSet.disjoint symmetry *)
-          - apply RegFile.eq_except_singleton.
-          - i. rewrite ORD1 in H. inv H.
-        }
-      * eauto.
-      * left. eapply paco7_mon; [apply sim_stmts_nil|]; ss.
-    + (* store *)
-      exploit sim_local_write; eauto.
-      { eapply Local.fulfill_step_future; eauto. }
-      i. des.
-      exploit reorder_fulfill_write; try apply x0; try apply STEP_SRC; eauto.
-      i. des.
-      eexists _, _, _, _, _, _. splits.
-      * econs 2; [|econs 1]. econs 4; eauto. econs. econs.
-      * econs. econs 4; eauto. econs.
-        { econs. }
-        { s. econs 1; eauto.
-          i. rewrite ORD1 in H. inv H.
-        }
-      * s. eauto.
-      * s. left. eapply paco7_mon; [apply sim_stmts_nil|]; ss.
-    + (* update *)
-      exploit sim_local_read; eauto.
-      { eapply Local.fulfill_step_future; eauto. }
-      i. des.
-      exploit sim_local_write; eauto.
-      { eapply Local.read_step_future; eauto.
-        eapply Local.fulfill_step_future; eauto.
+  - inversion PR. subst. i.
+    exploit (progress_step rs i2 nil); eauto.
+    i. des; [|by inv STEP; inv STATE; inv INSTR; inv REORDER].
+    destruct th2. exploit sim_store_step; eauto.
+    { econs 2. eauto. }
+    i. des.
+    + exploit internal_step_promise; eauto. i.
+      punfold SIM. exploit SIM; eauto; try reflexivity.
+      { exploit Thread.rtc_step_future; eauto. s. i. des.
+        exploit Thread.step_future; eauto. s. i. des. auto.
       }
-      { eapply Local.read_step_future; eauto. }
-      i. des.
-      exploit reorder_fulfill_read; try apply x0; try apply STEP_SRC; eauto. i. des.
-      exploit reorder_fulfill_write; try apply STEP2; try apply STEP_SRC0; eauto.
-      { eapply Local.read_step_future; eauto. }
-      i. des.
-      eexists _, _, _, _, _, _. splits.
-      * econs 2; [|econs 1]. econs 5; eauto. econs. econs. eauto.
-      * econs. econs 4; eauto.
-        { econs. econs. }
-        { s. econs 1. erewrite RegFile.eq_except_value; eauto.
-          - admit. (* RegSet.disjoint symmetry *)
-          - apply RegFile.eq_except_singleton.
-          - i. rewrite ORD1 in H. inv H.
-        }
-      * s. eauto.
-      * s. left. eapply paco7_mon; [apply sim_stmts_nil|]; ss.
-Admitted.
+      { exploit Thread.internal_step_future; eauto. s. i. des. auto. }
+      i. des. exploit PROMISE; eauto. i. des.
+      eexists _, _, _. splits; [|eauto].
+      etransitivity; eauto.
+      etransitivity; [econs 2; eauto|].
+      etransitivity; eauto.
+    + inv SIM. inv STEP; inv STATE.
+  - ii. exploit sim_store_step; eauto. i. des.
+    + eexists _, _, _, _, _, _. splits; eauto.
+      left. eapply paco7_mon; eauto. ss.
+    + eexists _, _, _, _, _, _. splits; eauto.
+Qed.
